Hacl.Poly1305.Field32xN.Lemmas*.fst: add interfaces
These files may needlessly constrain the build. Generally, having lemma
proofs in fstis is undesirable. There are many more cases, this is just
a start.

code/poly1305/Hacl.Poly1305.Field32xN.Lemmas0.fst
@@ -4,12 +4,11 @@ open Lib.IntTypes
 open Lib.IntVector
 open Lib.Sequence
 open FStar.Mul
-open FStar.Calc
 
 open Hacl.Spec.Poly1305.Vec
 include Hacl.Spec.Poly1305.Field32xN
 
-#reset-options "--z3rlimit 50"
+#set-options "--z3rlimit 50 --fuel 0 --ifuel 0"
 
 val lemma_prime: unit -> Lemma (pow2 130 % prime = 5)
 let lemma_prime () =
@@ -30,39 +29,16 @@ val lemma_mul5_distr_r: a:nat -> b:nat -> c:nat -> d:nat -> e:nat -> f:nat -> Le
   ((a + b + c + d + e) * f == a * f + b * f + c * f + d * f + e * f)
 let lemma_mul5_distr_r a b c d e f = ()
 
-
-val smul_mod_lemma:
-    #m1:scale32
-  -> #m2:scale32
-  -> a:nat{a <= m1 * max26}
-  -> b:nat{b <= m2 * max26} ->
-  Lemma (a * b % pow2 64 == a * b)
-
 let smul_mod_lemma #m1 #m2 a b =
   lemma_mult_le a (m1 * max26) b (m2 * max26);
   assert (a * b <= m1 * m2 * max26 * max26);
   FStar.Math.Lemmas.modulo_lemma (a * b) (pow2 64)
-
-
-val smul_add_mod_lemma:
-    #m1:scale32
-  -> #m2:scale32
-  -> #m3:scale64{m3 + m1 * m2 <= 4096}
-  -> a:nat{a <= m1 * max26}
-  -> b:nat{b <= m2 * max26}
-  -> c:nat{c <= m3 * max26 * max26} ->
-  Lemma ((c + a * b % pow2 64) % pow2 64 == c + a * b)
 
 let smul_add_mod_lemma #m1 #m2 #m3 a b c =
   assert_norm ((m3 + m1 * m2) * max26 * max26 < pow2 64);
   lemma_mult_le a (m1 * max26) b (m2 * max26);
   assert (c + a * b <= m3 * max26 * max26 + m1 * m2 * max26 * max26);
   FStar.Math.Lemmas.modulo_lemma (c + a * b) (pow2 64)
-
-
-val add5_lemma1: ma:scale64 -> mb:scale64 -> a:uint64 -> b:uint64 -> Lemma
-  (requires v a <= ma * max26 /\ v b <= mb * max26 /\ ma + mb <= 64)
-  (ensures  v (a +. b) == v a + v b /\ v (a +. b) <= (ma + mb) * max26)
 
 let add5_lemma1 ma mb a b =
   assert (v a + v b <= (ma + mb) * max26);
@@ -71,16 +47,7 @@ let add5_lemma1 ma mb a b =
   assert_norm (64 * max26 < pow2 32);
   Math.Lemmas.small_mod (v a + v b) (pow2 32)
 
-
-#set-options "--ifuel 1"
-
-val fadd5_eval_lemma_i:
-    #w:lanes
-  -> f1:felem5 w{felem_fits5 f1 (2,2,2,2,2)}
-  -> f2:felem5 w{felem_fits5 f2 (1,1,1,1,1)}
-  -> i:nat{i < w} ->
-  Lemma ((feval5 (fadd5 f1 f2)).[i] == pfadd (feval5 f1).[i] (feval5 f2).[i])
-
+#push-options "--ifuel 1"
 let fadd5_eval_lemma_i #w f1 f2 i =
   let o = fadd5 f1 f2 in
   let (f10, f11, f12, f13, f14) = as_tup64_i f1 i in
@@ -98,16 +65,7 @@ let fadd5_eval_lemma_i #w f1 f2 i =
     (as_nat5 (f10, f11, f12, f13, f14)) (as_nat5 (f20, f21, f22, f23, f24)) prime;
   FStar.Math.Lemmas.lemma_mod_plus_distr_r
     (as_nat5 (f10, f11, f12, f13, f14) % prime) (as_nat5 (f20, f21, f22, f23, f24)) prime
-
-
-val smul_felem5_fits_lemma_i:
-    #w:lanes
-  -> #m1:scale32
-  -> #m2:scale32
-  -> u1:uint64xN w{felem_fits1 u1 m1}
-  -> f2:uint64xN w{felem_fits1 f2 m2}
-  -> i:nat{i < w} ->
-  Lemma ((uint64xN_v (vec_mul_mod f2 u1)).[i] <= m1 * m2 * max26 * max26)
+#pop-options
 
 let smul_felem5_fits_lemma_i #w #m1 #m2 u1 f2 i =
   let o = vec_mul_mod f2 u1 in
@@ -115,16 +73,7 @@ let smul_felem5_fits_lemma_i #w #m1 #m2 u1 f2 i =
   assert ((uint64xN_v o).[i] == (uint64xN_v u1).[i] * (uint64xN_v f2).[i]);
   lemma_mult_le (uint64xN_v u1).[i] (m1 * max26) (uint64xN_v f2).[i] (m2 * max26)
 
-
-val smul_felem5_eval_lemma_i:
-    #w:lanes
-  -> #m1:scale32
-  -> #m2:scale32_5
-  -> u1:uint64xN w{felem_fits1 u1 m1}
-  -> f2:felem5 w{felem_fits5 f2 m2}
-  -> i:nat{i < w} ->
-  Lemma ((fas_nat5 (smul_felem5 #w u1 f2)).[i] == (uint64xN_v u1).[i] * (fas_nat5 f2).[i])
-
+#push-options "--ifuel 1"
 let smul_felem5_eval_lemma_i #w #m1 #m2 u1 f2 i =
   let o = smul_felem5 #w u1 f2 in
   let (m20, m21, m22, m23, m24) = m2 in
@@ -155,15 +104,7 @@ let smul_felem5_eval_lemma_i #w #m1 #m2 u1 f2 i =
     vu1 * v tf20 + vu1 * v tf21 * pow26 + vu1 * v tf22 * pow52 + vu1 * v tf23 * pow78 + vu1 * v tf24 * pow104;
     };
   assert (vu1 * (fas_nat5 f2).[i] == (fas_nat5 o).[i])
-
-
-val smul_felem5_fits_lemma1:
-    #w:lanes
-  -> #m1:scale32
-  -> #m2:scale32
-  -> u1:uint64xN w{felem_fits1 u1 m1}
-  -> f2:uint64xN w{felem_fits1 f2 m2} ->
-  Lemma (felem_wide_fits1 (vec_mul_mod f2 u1) (m1 * m2))
+#pop-options
 
 #push-options "--z3smtopt '(set-option :smt.arith.solver 2)'"
 // ^ much faster with solver 2, though it does work with solver 6 eventually
@@ -181,14 +122,6 @@ let smul_felem5_fits_lemma1 #w #m1 #m2 u1 f2 =
     smul_felem5_fits_lemma_i #w #m1 #m2 u1 f2 3
 #pop-options
 
-val smul_felem5_fits_lemma:
-    #w:lanes
-  -> #m1:scale32
-  -> #m2:scale32_5
-  -> u1:uint64xN w{felem_fits1 u1 m1}
-  -> f2:felem5 w{felem_fits5 f2 m2} ->
-  Lemma (felem_wide_fits5 (smul_felem5 #w u1 f2) (m1 *^ m2))
-
 let smul_felem5_fits_lemma #w #m1 #m2 u1 f2 =
   let (f20, f21, f22, f23, f24) = f2 in
   let (m20, m21, m22, m23, m24) = m2 in
@@ -198,32 +131,10 @@ let smul_felem5_fits_lemma #w #m1 #m2 u1 f2 =
   smul_felem5_fits_lemma1 #w #m1 #m23 u1 f23;
   smul_felem5_fits_lemma1 #w #m1 #m24 u1 f24
 
-
-val smul_felem5_eval_lemma:
-    #w:lanes
-  -> #m1:scale32
-  -> #m2:scale32_5
-  -> u1:uint64xN w{felem_fits1 u1 m1}
-  -> f2:felem5 w{felem_fits5 f2 m2} ->
-  Lemma (fas_nat5 (smul_felem5 #w u1 f2) ==
-    map2 #nat #nat #nat (fun a b -> a * b) (uint64xN_v u1) (fas_nat5 f2))
-
 let smul_felem5_eval_lemma #w #m1 #m2 u1 f2 =
   FStar.Classical.forall_intro (smul_felem5_eval_lemma_i #w #m1 #m2 u1 f2);
   eq_intro (fas_nat5 (smul_felem5 #w u1 f2))
     (map2 #nat #nat #nat (fun a b -> a * b) (uint64xN_v u1) (fas_nat5 f2))
-
-
-val smul_add_felem5_fits_lemma_i:
-    #w:lanes
-  -> #m1:scale32
-  -> #m2:scale32
-  -> #m3:scale64{m3 + m1 * m2 <= 4096}
-  -> u1:uint64xN w{felem_fits1 u1 m1}
-  -> f2:uint64xN w{felem_fits1 f2 m2}
-  -> acc1:uint64xN w{felem_wide_fits1 acc1 m3}
-  -> i:nat{i < w} ->
-  Lemma ((uint64xN_v (vec_add_mod acc1 (vec_mul_mod f2 u1))).[i] <= (m3 + m1 * m2) * max26 * max26)
 
 #push-options "--z3rlimit 250"
 let smul_add_felem5_fits_lemma_i #w #m1 #m2 #m3 u1 f2 acc1 i =
@@ -234,18 +145,7 @@ let smul_add_felem5_fits_lemma_i #w #m1 #m2 #m3 u1 f2 acc1 i =
   assert ((uint64xN_v o).[i] <= m3 * max26 * max26 + m1 * m2 * max26 * max26)
 #pop-options
 
-val smul_add_felem5_eval_lemma_i:
-    #w:lanes
-  -> #m1:scale32
-  -> #m2:scale32_5
-  -> #m3:scale64_5{m3 +* m1 *^ m2 <=* s64x5 4096}
-  -> u1:uint64xN w{felem_fits1 u1 m1}
-  -> f2:felem5 w{felem_fits5 f2 m2}
-  -> acc1:felem_wide5 w{felem_wide_fits5 acc1 m3}
-  -> i:nat{i < w} ->
-  Lemma ((fas_nat5 (smul_add_felem5 #w u1 f2 acc1)).[i] ==
-    (fas_nat5 acc1).[i] + (uint64xN_v u1).[i] * (fas_nat5 f2).[i])
-
+#push-options "--ifuel 1"
 let smul_add_felem5_eval_lemma_i #w #m1 #m2 #m3 u1 f2 acc1 i =
   let o = smul_add_felem5 #w u1 f2 acc1 in
   let (m20, m21, m22, m23, m24) = m2 in
@@ -293,17 +193,7 @@ let smul_add_felem5_eval_lemma_i #w #m1 #m2 #m3 u1 f2 acc1 i =
     vu1 * v tf20 + vu1 * v tf21 * pow26 + vu1 * v tf22 * pow52 + vu1 * v tf23 * pow78 + vu1 * v tf24 * pow104;
     };
   assert ((fas_nat5 o).[i] == (fas_nat5 acc1).[i] + vu1 * (fas_nat5 f2).[i])
-
-
-val smul_add_felem5_fits_lemma1:
-    #w:lanes
-  -> #m1:scale32
-  -> #m2:scale32
-  -> #m3:scale64{m3 + m1 * m2 <= 4096}
-  -> u1:uint64xN w{felem_fits1 u1 m1}
-  -> f2:uint64xN w{felem_fits1 f2 m2}
-  -> acc1:uint64xN w{felem_wide_fits1 acc1 m3} ->
-  Lemma (felem_wide_fits1 (vec_add_mod acc1 (vec_mul_mod f2 u1)) (m3 + m1 * m2))
+#pop-options
 
 #push-options "--z3smtopt '(set-option :smt.arith.solver 2)'"
 // ^ much faster with solver 2
@@ -321,16 +211,6 @@ let smul_add_felem5_fits_lemma1 #w #m1 #m2 #m3 u1 f2 acc1 =
     smul_add_felem5_fits_lemma_i #w #m1 #m2 #m3 u1 f2 acc1 3
 #pop-options
 
-val smul_add_felem5_fits_lemma:
-    #w:lanes
-  -> #m1:scale32
-  -> #m2:scale32_5
-  -> #m3:scale64_5{m3 +* m1 *^ m2 <=* s64x5 4096}
-  -> u1:uint64xN w{felem_fits1 u1 m1}
-  -> f2:felem5 w{felem_fits5 f2 m2}
-  -> acc1:felem_wide5 w{felem_wide_fits5 acc1 m3} ->
-  Lemma (felem_wide_fits5 (smul_add_felem5 #w u1 f2 acc1) (m3 +* m1 *^ m2))
-
 let smul_add_felem5_fits_lemma #w #m1 #m2 #m3 u1 f2 acc1 =
   let (f20, f21, f22, f23, f24) = f2 in
   let (m20, m21, m22, m23, m24) = m2 in
@@ -342,31 +222,12 @@ let smul_add_felem5_fits_lemma #w #m1 #m2 #m3 u1 f2 acc1 =
   smul_add_felem5_fits_lemma1 #w #m1 #m23 #m33 u1 f23 a3;
   smul_add_felem5_fits_lemma1 #w #m1 #m24 #m34 u1 f24 a4
 
-
-val smul_add_felem5_eval_lemma:
-    #w:lanes
-  -> #m1:scale32
-  -> #m2:scale32_5
-  -> #m3:scale64_5{m3 +* m1 *^ m2 <=* s64x5 4096}
-  -> u1:uint64xN w{felem_fits1 u1 m1}
-  -> f2:felem5 w{felem_fits5 f2 m2}
-  -> acc1:felem_wide5 w{felem_wide_fits5 acc1 m3} ->
-  Lemma (fas_nat5 (smul_add_felem5 #w u1 f2 acc1) ==
-    map2 #nat #nat #nat (fun a b -> a + b) (fas_nat5 acc1)
-      (map2 #nat #nat #nat (fun a b -> a * b) (uint64xN_v u1) (fas_nat5 f2)))
-
 let smul_add_felem5_eval_lemma #w #m1 #m2 #m3 u1 f2 acc1 =
   let tmp =
     map2 #nat #nat #nat (fun a b -> a + b) (fas_nat5 acc1)
       (map2 #nat #nat #nat (fun a b -> a * b) (uint64xN_v u1) (fas_nat5 f2)) in
   FStar.Classical.forall_intro (smul_add_felem5_eval_lemma_i #w #m1 #m2 #m3 u1 f2 acc1);
   eq_intro (fas_nat5 (smul_add_felem5 #w u1 f2 acc1)) tmp
-
-
-val lemma_fmul5_pow26: r:tup64_5 -> Lemma
-  (requires (let (r0, r1, r2, r3, r4) = r in v r4 * 5 <= 10 * pow26))
-  (ensures  (let (r0, r1, r2, r3, r4) = r in
-    (pow26 * as_nat5 r) % prime == as_nat5 (r4 *! u64 5, r0, r1, r2, r3) % prime))
 
 let lemma_fmul5_pow26 r =
   let (r0, r1, r2, r3, r4) = r in
@@ -398,13 +259,6 @@ let lemma_fmul5_pow26 r =
   assert ((pow26 * as_nat5 r) % prime ==
     (v r0 * pow26 + v r1 * pow52 + v r2 * pow78 + v r3 * pow104 + v r4 * 5) % prime)
 
-
-val lemma_fmul5_pow52: r:tup64_5 -> Lemma
-  (requires (let (r0, r1, r2, r3, r4) = r in
-    v r4 * 5 <= 10 * pow26 /\ v r3 * 5 <= 10 * pow26))
-  (ensures (let (r0, r1, r2, r3, r4) = r in
-    (pow52 * as_nat5 r) % prime == as_nat5 (r3 *! u64 5, r4 *! u64 5, r0, r1, r2) % prime))
-
 let lemma_fmul5_pow52 r =
   let (r0, r1, r2, r3, r4) = r in
   calc (==) {
@@ -423,13 +277,6 @@ let lemma_fmul5_pow52 r =
     as_nat5 (r3 *! u64 5, r4 *! u64 5, r0, r1, r2) % prime;
   };
   assert ((pow52 * as_nat5 r) % prime == as_nat5 (r3 *! u64 5, r4 *! u64 5, r0, r1, r2) % prime)
-
-
-val lemma_fmul5_pow78: r:tup64_5 -> Lemma
-  (requires (let (r0, r1, r2, r3, r4) = r in
-    v r4 * 5 <= 10 * pow26 /\ v r3 * 5 <= 10 * pow26 /\ v r2 * 5 <= 10 * pow26))
-  (ensures (let (r0, r1, r2, r3, r4) = r in
-    (pow78 * as_nat5 r) % prime == as_nat5 (r2 *! u64 5, r3 *! u64 5, r4 *! u64 5, r0, r1) % prime))
 
 let lemma_fmul5_pow78 r =
   let (r0, r1, r2, r3, r4) = r in
@@ -450,14 +297,6 @@ let lemma_fmul5_pow78 r =
   };
   assert ((pow78 * as_nat5 r) % prime == as_nat5 (r2 *! u64 5, r3 *! u64 5, r4 *! u64 5, r0, r1) % prime)
 
-
-val lemma_fmul5_pow104: r:tup64_5 -> Lemma
-  (requires (let (r0, r1, r2, r3, r4) = r in
-    v r4 * 5 <= 10 * pow26 /\ v r3 * 5 <= 10 * pow26 /\
-    v r2 * 5 <= 10 * pow26 /\ v r1 * 5 <= 10 * pow26))
-  (ensures (let (r0, r1, r2, r3, r4) = r in
-    (pow104 * as_nat5 r) % prime == as_nat5 (r1 *! u64 5, r2 *! u64 5, r3 *! u64 5, r4 *! u64 5, r0) % prime))
-
 let lemma_fmul5_pow104 r =
   let (r0, r1, r2, r3, r4) = r in
   calc (==) {
@@ -476,18 +315,6 @@ let lemma_fmul5_pow104 r =
     as_nat5 (r1 *! u64 5, r2 *! u64 5, r3 *! u64 5, r4 *! u64 5, r0) % prime;
   };
   assert ((pow104 * as_nat5 r) % prime == as_nat5 (r1 *! u64 5, r2 *! u64 5, r3 *! u64 5, r4 *! u64 5, r0) % prime)
-
-
-val mul_felem5_lemma_1:
-    f1:tup64_5{tup64_fits5 f1 (3, 3, 3, 3, 3)}
-  -> r:tup64_5{tup64_fits5 r (2, 2, 2, 2, 2)} ->
-  Lemma
-  (let (f10, f11, f12, f13, f14) = f1 in
-  let (r0, r1, r2, r3, r4) = r in
-  (as_nat5 f1 * as_nat5 r) % prime ==
-  (v f10 * as_nat5 r +
-   v f11 * as_nat5 (r4 *! u64 5, r0, r1, r2, r3) +
-   v f12 * pow52 * as_nat5 r + v f13 * pow78 * as_nat5 r + v f14 * pow104 * as_nat5 r) % prime)
 
 let mul_felem5_lemma_1 f1 r =
   let (f10, f11, f12, f13, f14) = f1 in
@@ -516,19 +343,6 @@ let mul_felem5_lemma_1 f1 r =
     };
   assert ((as_nat5 f1 * as_nat5 r) % prime == (tmp + v f11 * as_nat5 (r4 *! u64 5, r0, r1, r2, r3)) % prime)
 
-
-val mul_felem5_lemma_2:
-    f1:tup64_5{tup64_fits5 f1 (3, 3, 3, 3, 3)}
-  -> r:tup64_5{tup64_fits5 r (2, 2, 2, 2, 2)} ->
-  Lemma
-  (let (f10, f11, f12, f13, f14) = f1 in
-  let (r0, r1, r2, r3, r4) = r in
-  (as_nat5 f1 * as_nat5 r) % prime ==
-  (v f10 * as_nat5 r +
-   v f11 * as_nat5 (r4 *! u64 5, r0, r1, r2, r3) +
-   v f12 * as_nat5 (r3 *! u64 5, r4 *! u64 5, r0, r1, r2) +
-   v f13 * pow78 * as_nat5 r + v f14 * pow104 * as_nat5 r) % prime)
-
 let mul_felem5_lemma_2 f1 r =
   let (f10, f11, f12, f13, f14) = f1 in
   let (r0, r1, r2, r3, r4) = r in
@@ -554,20 +368,6 @@ let mul_felem5_lemma_2 f1 r =
     (tmp + v f12 * as_nat5 (r3 *! u64 5, r4 *! u64 5, r0, r1, r2)) % prime;
    };
   assert ((as_nat5 f1 * as_nat5 r) % prime == (tmp + v f12 * as_nat5 (r3 *! u64 5, r4 *! u64 5, r0, r1, r2)) % prime)
-
-
-val mul_felem5_lemma_3:
-    f1:tup64_5{tup64_fits5 f1 (3, 3, 3, 3, 3)}
-  -> r:tup64_5{tup64_fits5 r (2, 2, 2, 2, 2)} ->
-  Lemma
-  (let (f10, f11, f12, f13, f14) = f1 in
-  let (r0, r1, r2, r3, r4) = r in
-  (as_nat5 f1 * as_nat5 r) % prime ==
-  (v f10 * as_nat5 r +
-   v f11 * as_nat5 (r4 *! u64 5, r0, r1, r2, r3) +
-   v f12 * as_nat5 (r3 *! u64 5, r4 *! u64 5, r0, r1, r2) +
-   v f13 * as_nat5 (r2 *! u64 5, r3 *! u64 5, r4 *! u64 5, r0, r1) +
-   v f14 * pow104 * as_nat5 r) % prime)
 
 let mul_felem5_lemma_3 f1 r =
   let (f10, f11, f12, f13, f14) = f1 in
@@ -595,20 +395,6 @@ let mul_felem5_lemma_3 f1 r =
    };
   assert ((as_nat5 f1 * as_nat5 r) % prime == (tmp + v f13 * as_nat5 (r2 *! u64 5, r3 *! u64 5, r4 *! u64 5, r0, r1)) % prime)
 
-
-val mul_felem5_lemma_4:
-    f1:tup64_5{tup64_fits5 f1 (3, 3, 3, 3, 3)}
-  -> r:tup64_5{tup64_fits5 r (2, 2, 2, 2, 2)} ->
-  Lemma
-  (let (f10, f11, f12, f13, f14) = f1 in
-  let (r0, r1, r2, r3, r4) = r in
-  (as_nat5 f1 * as_nat5 r) % prime ==
-  (v f10 * as_nat5 r +
-   v f11 * as_nat5 (r4 *! u64 5, r0, r1, r2, r3) +
-   v f12 * as_nat5 (r3 *! u64 5, r4 *! u64 5, r0, r1, r2) +
-   v f13 * as_nat5 (r2 *! u64 5, r3 *! u64 5, r4 *! u64 5, r0, r1) +
-   v f14 * as_nat5 (r1 *! u64 5, r2 *! u64 5, r3 *! u64 5, r4 *! u64 5, r0)) % prime)
-
 let mul_felem5_lemma_4 f1 r =
   let (f10, f11, f12, f13, f14) = f1 in
   let (r0, r1, r2, r3, r4) = r in
@@ -635,41 +421,12 @@ let mul_felem5_lemma_4 f1 r =
    };
   assert ((as_nat5 f1 * as_nat5 r) % prime == (tmp + v f14 * as_nat5 (r1 *! u64 5, r2 *! u64 5, r3 *! u64 5, r4 *! u64 5, r0)) % prime)
 
-
-val mul_felem5_lemma:
-    f1:tup64_5{tup64_fits5 f1 (3, 3, 3, 3, 3)}
-  -> r:tup64_5{tup64_fits5 r (2, 2, 2, 2, 2)} ->
-  Lemma
-    (let (f10, f11, f12, f13, f14) = f1 in
-    let (r0, r1, r2, r3, r4) = r in
-    (as_pfelem5 f1) `pfmul` (as_pfelem5 r) ==
-    (v f10 * as_nat5 (r0, r1, r2, r3, r4) +
-    v f11 * as_nat5 (r4 *! u64 5, r0, r1, r2, r3) +
-    v f12 * as_nat5 (r3 *! u64 5, r4 *! u64 5, r0, r1, r2) +
-    v f13 * as_nat5 (r2 *! u64 5, r3 *! u64 5, r4 *! u64 5, r0, r1) +
-    v f14 * as_nat5 (r1 *! u64 5, r2 *! u64 5, r3 *! u64 5, r4 *! u64 5, r0)) % prime)
-
 let mul_felem5_lemma f1 r =
   let (f10, f11, f12, f13, f14) = f1 in
   let (r0, r1, r2, r3, r4) = r in
   mul_felem5_lemma_4 f1 r;
   FStar.Math.Lemmas.lemma_mod_mul_distr_l (as_nat5 f1) (as_nat5 r) prime;
   FStar.Math.Lemmas.lemma_mod_mul_distr_r (as_nat5 f1 % prime) (as_nat5 r) prime
-
-
-val precomp_r5_as_tup64:
-    #w:lanes
-  -> r:felem5 w{felem_fits5 r (2, 2, 2, 2, 2)}
-  -> i:nat{i < w} ->
-  Lemma
-  (let r5 = precomp_r5 r in
-   let (tr50, tr51, tr52, tr53, tr54) = as_tup64_i r5 i in
-   let (tr0, tr1, tr2, tr3, tr4) = as_tup64_i r i in
-   tr50 == tr0 *! u64 5 /\
-   tr51 == tr1 *! u64 5 /\
-   tr52 == tr2 *! u64 5 /\
-   tr53 == tr3 *! u64 5 /\
-   tr54 == tr4 *! u64 5)
 
 let precomp_r5_as_tup64 #w r i =
   let r5 = precomp_r5 r in
@@ -688,30 +445,6 @@ let precomp_r5_as_tup64 #w r i =
   assert (v tr52 == v (tr2 *! u64 5));
   assert (v tr53 == v (tr3 *! u64 5));
   assert (v tr54 == v (tr4 *! u64 5))
-
-
-val mul_felem5_eval_as_tup64:
-    #w:lanes
-  -> f1:felem5 w{felem_fits5 f1 (3, 3, 3, 3, 3)}
-  -> r:felem5 w{felem_fits5 r (2, 2, 2, 2, 2)}
-  -> r5:felem5 w{felem_fits5 r5 (10, 10, 10, 10, 10) /\ r5 == precomp_r5 r}
-  -> i:nat{i < w} ->
-  Lemma
-  (let (r0, r1, r2, r3, r4) = r in
-   let (f10, f11, f12, f13, f14) = f1 in
-   let (r50, r51, r52, r53, r54) = r5 in
-   let (tr0, tr1, tr2, tr3, tr4) = as_tup64_i r i in
-   let (tf10, tf11, tf12, tf13, tf14) = as_tup64_i f1 i in
-  (uint64xN_v f10).[i] * (fas_nat5 (r0,r1,r2,r3,r4)).[i] +
-  (uint64xN_v f11).[i] * (fas_nat5 (r54,r0,r1,r2,r3)).[i] +
-  (uint64xN_v f12).[i] * (fas_nat5 (r53,r54,r0,r1,r2)).[i] +
-  (uint64xN_v f13).[i] * (fas_nat5 (r52,r53,r54,r0,r1)).[i] +
-  (uint64xN_v f14).[i] * (fas_nat5 (r51,r52,r53,r54,r0)).[i] ==
-  (v tf10 * as_nat5 (tr0, tr1, tr2, tr3, tr4) +
-   v tf11 * as_nat5 (tr4 *! u64 5, tr0, tr1, tr2, tr3) +
-   v tf12 * as_nat5 (tr3 *! u64 5, tr4 *! u64 5, tr0, tr1, tr2) +
-   v tf13 * as_nat5 (tr2 *! u64 5, tr3 *! u64 5, tr4 *! u64 5, tr0, tr1) +
-   v tf14 * as_nat5 (tr1 *! u64 5, tr2 *! u64 5, tr3 *! u64 5, tr4 *! u64 5, tr0)))
 
 let mul_felem5_eval_as_tup64 #w f1 r r5 i =
   let (r0, r1, r2, r3, r4) = r in
